src/tls/Signature.fst
@@ -1,16 +1,13 @@
 module Signature
+
 module HS = FStar.HyperStack //Added automatically
 module HST = FStar.HyperStack.ST //Added automatically
-
-
 open FStar.HyperStack
 
 open FStar.Monotonic.Seq
-
 open FStar.Bytes
 open CoreCrypto
 open Hashing.Spec // masking CoreCrypto's hashAlg
-
 open TLSConstants
 open Cert
 
@@ -93,7 +90,7 @@ abstract let evolves (#a:alg) (s1:state a) (s2:state a) =
 let lemma_evolves_monotone (#a:alg): Lemma (monotonic (state a) (evolves #a)) =
   FStar.Classical.forall_intro (seq_extension_reflexive #(signed a));
   FStar.Classical.forall_intro_3 (grows_transitive #(signed a))
-
+ sdfsdfsdfsd
 private val st_update: #a:alg
   -> s1:state a
   -> signed a
