src/tls/TLSError.fst
@@ -1,5 +1,5 @@
 ﻿module TLSError
-open FStar.String
+
 (* TLS explicitly returns run-time errors:
    results carry either values or error descriptions *)
 
